revert QUIC.Spec.fsti

src/QUIC.Spec.fsti
@@ -6,7 +6,6 @@ open Model.Indexing
 module S = FStar.Seq
 module HD = Spec.Hash.Definitions
 module AEAD = Spec.Agile.AEAD
-module Cipher = Spec.Agile.Cipher
 
 // JP: should we allow inversion on either hash algorithm or AEAD algorithm?
 #set-options "--max_fuel 0 --max_ifuel 0"
@@ -42,10 +41,11 @@ type pbytes' (is_retry: bool) = b:bytes{let l = S.length b in if is_retry then l
 type cbytes = b:bytes{let l = S.length b in 19 <= l /\ l < max_cipher_length}
 type cbytes' (is_retry: bool) = b: bytes { let l = S.length b in if is_retry then l == 0 else (19 <= l /\ l < max_cipher_length) }
 
+// JP: this is Spec.Agile.Cipher.key_length
 let ae_keysize (a:ea) =
-  Spec.Agile.AEAD.key_length a
-let cipher_keysize (a:ea) =
-  Spec.Agile.Cipher.key_length (Spec.Agile.AEAD.cipher_alg_of_supported_alg a)
+  match a with
+  | AEAD.AES128_GCM -> 16
+  | _ -> 32
 
 // Static byte sequences to be fed into secret derivation. Marked as inline, so
 // that they can be used as arguments to gcmalloc_of_list for top-level arrays.
@@ -58,7 +58,7 @@ val label_hp: lbytes 2
 
 val derive_secret:
   a: ha ->
-  prk: Spec.Hash.Definitions.bytes_hash a ->
+  prk:Spec.Hash.Definitions.bytes_hash a ->
   label: bytes ->
   len: nat ->
   Pure (lbytes len)
@@ -80,14 +80,9 @@ type qbytes (n:nat4) = lbytes (add3 n)
 // JP: seems appropriate for this module...?
 let _: squash (inversion header) = allow_inversion header
 
-inline_for_extraction
-val pn_sizemask_naive: pn_len:nat2 -> lbytes (pn_len + 1)
-
-val block_of_sample: a:Spec.Agile.Cipher.cipher_alg -> k: Spec.Agile.Cipher.key a -> sample: lbytes 16 -> lbytes 16
-
 // Header protection only
 val header_encrypt: a:ea ->
-  hpk: lbytes (cipher_keysize a) ->
+  hpk: lbytes (ae_keysize a) ->
   h: header ->
   c: cbytes' (is_retry h) ->
   GTot packet
@@ -106,7 +101,7 @@ type h_result =
 
 // Note that cid_len cannot be parsed from short headers
 val header_decrypt: a:ea ->
-  hpk: lbytes (cipher_keysize a) ->
+  hpk: lbytes (ae_keysize a) ->
   cid_len: nat { cid_len <= 20 } ->
   last: nat { last + 1 < pow2 62 } ->
   p: packet ->
@@ -130,7 +125,7 @@ module U64 = FStar.UInt64
 // of the same arguments (see QUIC.Spec.Old.*_malleable)
 val lemma_header_encryption_correct:
   a:ea ->
-  k:lbytes (cipher_keysize a) ->
+  k:lbytes (ae_keysize a) ->
   h:header ->
   cid_len: nat { cid_len <= 20 /\ (MShort? h ==> cid_len == dcid_len h) } ->
   last: nat { last + 1 < pow2 62 /\ ((~ (is_retry h)) ==> in_window (U32.v (pn_length h) - 1) last (U64.v (packet_number h))) } ->
@@ -151,14 +146,12 @@ type result =
 
 val encrypt:
   a: ea ->
-  k: lbytes (ae_keysize a) ->
+  k: lbytes (AEAD.key_length a) ->
   static_iv: lbytes 12 ->
-  hpk: lbytes (cipher_keysize a) ->
+  hpk: lbytes (ae_keysize a) ->
   h: header ->
-  plain: pbytes' (is_retry h) ->
-  Ghost packet
-  (requires has_payload_length h ==> U64.v (payload_length h) == S.length plain + AEAD.tag_length a)
-  (ensures fun _ -> True)
+  plain: pbytes' (is_retry h) { has_payload_length h ==> U64.v (payload_length h) == S.length plain + AEAD.tag_length a } ->
+  GTot packet
 
 /// decryption and correctness
 
@@ -166,9 +159,9 @@ val encrypt:
 
 val decrypt:
   a: ea ->
-  k: lbytes (ae_keysize a) ->
+  k: lbytes (AEAD.key_length a) ->
   static_iv: lbytes 12 ->
-  hpk: lbytes (cipher_keysize a) ->
+  hpk: lbytes (ae_keysize a) ->
   last: nat{last+1 < pow2 62} ->
   cid_len: nat { cid_len <= 20 } ->
   packet: packet ->
@@ -183,9 +176,9 @@ val decrypt:
 
 val lemma_encrypt_correct:
   a: ea ->
-  k: lbytes (ae_keysize a) ->
+  k: lbytes (AEAD.key_length a) ->
   siv: lbytes 12 ->
-  hpk: lbytes (cipher_keysize a) ->
+  hpk: lbytes (ae_keysize a) ->
   h: header ->
   cid_len: nat { cid_len <= 20 /\ (MShort? h ==> cid_len == dcid_len h) } ->
   last: nat{last+1 < pow2 62 } ->
